feat(na): na_inv_P not Timeless and Persistant anymore

theories/rust_typing/existentials_na.v
@@ -9,8 +9,7 @@ Record na_ex_inv_def `{!typeGS Σ} (X : Type) (Y : Type) : Type := na_mk_ex_inv_
 
   na_inv_P_lfts : list lft;
   na_inv_P_wf_E : elctx;
-  na_inv_P_pers : ∀ π x y, Persistent (na_inv_P π x y);
-  na_inv_P_timeless : ∀ π x y, Timeless (na_inv_P π x y);
+  (* na_inv_P_timeless : ∀ π x y, Timeless (na_inv_P π x y); *)
 }.
 
 (* Stop Typeclass resolution for the [inv_P_pers] argument, to make it more deterministic. *)
@@ -19,33 +18,26 @@ Definition na_mk_ex_inv_def `{!typeGS Σ} {X Y : Type}
 
   inv_P_lfts
   (inv_P_wf_E : elctx)
-  (inv_P_pers : TCNoResolve (∀ (π : thread_id) (x : X) (y : Y), Persistent (inv_P π x y)))
-  (inv_P_timeless: TCNoResolve (∀ (π : thread_id) (x : X) (y : Y), Timeless (inv_P π x y)))
+  (* (inv_P_timeless: TCNoResolve (∀ (π : thread_id) (x : X) (y : Y), Timeless (inv_P π x y))) *)
 
   := na_mk_ex_inv_def' _ _ _ _
-       inv_P inv_P_lfts inv_P_wf_E inv_P_pers inv_P_timeless.
+       inv_P inv_P_lfts inv_P_wf_E (* inv_P_timeless *).
 
 Global Arguments na_inv_P {_ _ _ _}.
 Global Arguments na_inv_P_lfts {_ _ _ _}.
 Global Arguments na_inv_P_wf_E {_ _ _ _}.
-Global Arguments na_inv_P_pers {_ _ _ _}.
-Global Arguments na_inv_P_timeless {_ _ _ _}.
-Global Existing Instance na_inv_P_pers.
-Global Existing Instance na_inv_P_timeless.
+(* Global Arguments na_inv_P_timeless {_ _ _ _}. *)
+(* Global Existing Instance na_inv_P_timeless. *)
 Global Typeclasses Opaque na_mk_ex_inv_def.
 
 (** Smart constructor for persistent and timeless [P] *)
 Program Definition na_mk_pers_ex_inv_def
   `{!typeGS Σ} {X : Type} {Y : Type} (P : X → Y → iProp Σ)
-  (_: TCNoResolve (∀ x y, Persistent (P x y)))
-  (_: TCNoResolve (∀ x y, Timeless (P x y))): na_ex_inv_def X Y :=
-    na_mk_ex_inv_def (λ _, P) [] [] _ _.
-Next Obligation.
-  by rewrite /TCNoResolve.
-Qed.
-Next Obligation.
-  by rewrite /TCNoResolve.
-Qed.
+  (* (_: TCNoResolve (∀ x y, Timeless (P x y))): na_ex_inv_def X Y *) :=
+    na_mk_ex_inv_def (λ _, P) [] [] (* _ *).
+(* Next Obligation. *)
+(*   by rewrite /TCNoResolve. *)
+(* Qed. *)
 
 Global Typeclasses Opaque na_mk_pers_ex_inv_def.
 
@@ -55,10 +47,10 @@ Section na_ex.
 
   Program Definition na_ex_plain_t (ty : type X) : type Y := {|
     ty_own_val π r v := ∃ x : X, P.(na_inv_P) π x r ∗ ty.(ty_own_val) π x v;
-    ty_shr κ π r l := ∃ x : X,
-      P.(na_inv_P) π x r ∗
+    ty_shr κ π r l :=
+      (* TODO: Add persistant part that cannot depends on the refined value *)
       ty.(ty_sidecond) ∗
-      &na{κ, π, shrN.@l}(∃ v, l ↦ v ∗ ty.(ty_own_val) π x v) ∗
+      &na{κ, π, shrN.@l}(∃ x, l ↦: ty.(ty_own_val) π x ∗ P.(na_inv_P) π x r) ∗
       (∃ ly : layout, ⌜l `has_layout_loc` ly⌝ ∗ ⌜syn_type_has_layout (ty_syn_type ty) ly⌝);
 
     ty_syn_type := ty.(ty_syn_type);
@@ -90,64 +82,66 @@ Section na_ex.
 
   (* ty_shr_sidecond *)
   Next Obligation.
-    iIntros (?????) "(% & (_ & $ & _))".
+    iIntros (?????) "($ & _ & _)".
   Qed.
 
   (* ty_shr_aligned *)
   Next Obligation.
-    iIntros (?????) "(% & _ & _ & _ & $)".
+    iIntros (?????) "(_ & _ & $)".
   Qed.
 
   (* ty_share *)
   Next Obligation.
-    iIntros (ty E κ l ly π r q ?) "#(LFT & TIME & LLCTX) Htok %Halg %Hly Hlb Hb".
-    setoid_rewrite bi.sep_exist_l at 1.
-    setoid_rewrite bi_exist_comm at 1.
+    iIntros (ty E κ l ly π r q ?) "#(LFT & TIME & LLCTX) Htok %Halg %Hly Hlb Hbor".
+    iEval (setoid_rewrite bi.sep_exist_l) in "Hbor".
+    iEval (setoid_rewrite bi_exist_comm) in "Hbor".
 
     rewrite lft_intersect_list_app -!lft_tok_sep.
     iDestruct "Htok" as "(Htok & ? & ?)".
 
-    iApply fupd_logical_step.
-    iMod (bor_exists_tok with "LFT Hb Htok") as "(%x & Hb & Htok)"; first solve_ndisj.
+    iApply fupd_logical_step; iApply logical_step_intro.
+    iMod (bor_exists_tok with "LFT Hbor Htok") as "(%x & Hbor & Htok)"; first solve_ndisj.
 
-    iPoseProof (bor_iff _ _ (P.(na_inv_P) π x r ∗ (∃ a : val, l ↦ a ∗ a ◁ᵥ{ π} x @ ty)) with "[] Hb") as "Hb".
+    (* NOTE: Is there a simplier setoid_rewrite to do here ? *)
+    iPoseProof (bor_iff _ _ (P.(na_inv_P) π x r ∗ l ↦: ty_own_val ty π x) with "[] Hbor") as "Hbor".
     { iNext. iModIntro. iSplit; [iIntros "(% & ? & ? & ?)" | iIntros "(? & (% & ? & ?))"]; eauto with iFrame. }
 
-    iMod (bor_sep with "LFT Hb") as "(HP & Hb)"; first solve_ndisj.
-    iMod (bor_persistent with "LFT HP Htok") as "(>HP & Htok)"; first solve_ndisj.
+    iMod (bor_sep with "LFT Hbor") as "(Hinv & Hbor)"; first solve_ndisj.
+    iMod (bor_get_persistent _ (ty_sidecond ty) with "LFT [] Hbor Htok") as "(Hty & Hbor & Htok)"; first solve_ndisj.
+    { iIntros "Hl".
+      iDestruct "Hl" as (v) "(Hl & Hv)".
 
-    iMod (bor_get_persistent _ (ty_sidecond ty) with "LFT [] Hb Htok") as "(Hty & Hb & Htok)"; first solve_ndisj.
-    { iIntros "$ !> !>".
-      iApply ty_own_val_sidecond.
-      (* NOTE: Use ty_own_val_sidecond *)
+      (* NOTE: ty_own_val_sidecond *)
       admit. }
 
-    iMod (bor_na with "Hb") as "Hb"; first solve_ndisj.
-    iModIntro.
+    iMod (bor_combine with "LFT Hbor Hinv") as "Hbor"; first solve_ndisj.
+    iMod (bor_na with "Hbor") as "Hbor"; first solve_ndisj.
 
-    iApply logical_step_intro; iFrame.
-    iExists x; eauto with iFrame.
+    iModIntro; iFrame.
+    iSplitL "Hbor". { admit. }
+    iExists ly; eauto with iFrame.
   Admitted.
 
   (* ty_shr_mono *)
   Next Obligation.
-    iIntros (ty κ κ' π r l) "#Hincl (%x & HP & Hty & Hshr& Hly)".
-    iExists x. iFrame.
-    iApply (na_bor_shorten with "Hincl Hshr").
+    iIntros (ty κ κ' π r l) "Hincl ($ & Hbor & %ly & ? & ?)".
+    iSplitL "Hincl Hbor".
+    - iApply (na_bor_shorten with "Hincl Hbor").
+    - iExists ly. iFrame.
   Qed.
 
   (* ty_own_ghost_drop *)
   Next Obligation.
-    iIntros (ty π r v F ?) "(%x & HP & Ha)".
-    iPoseProof (ty_own_ghost_drop with "Ha") as "Ha"; first done.
-    iApply (logical_step_compose with "Ha").
+    iIntros (ty π r v F ?) "(%x & ? & Hv)".
+    iPoseProof (ty_own_ghost_drop with "Hv") as "Hv"; first done.
+    iApply (logical_step_compose with "Hv").
     iApply logical_step_intro.
-    iIntros "Hdrop". eauto with iFrame.
+    iIntros "?". eauto with iFrame.
   Qed.
 
   (* _ty_memcast_compat *)
   Next Obligation.
-    iIntros (ty ot mt st π r v Hot) "(%x & HP & Hv)".
+    iIntros (ty ot mt st π r v Hot) "(%x & ? & Hv)".
     iPoseProof (ty_memcast_compat with "Hv") as "Hm"; first done.
     destruct mt; eauto with iFrame.
   Qed.
@@ -243,10 +237,8 @@ Section generated_code.
     Program Definition Cell_inv_t_inv_spec : na_ex_inv_def (Cell_rt) (Z) :=
       na_mk_ex_inv_def
         (λ π inner_rfn 'x, ⌜inner_rfn = -[#(x)]⌝ ∗ ⌜Zeven x⌝ ∗ True)%I
-        []
-        [] _ _.
-    Next Obligation. ex_t_solve_persistent. Qed.
-    Next Obligation. ex_t_solve_timeless. Qed.
+        [] [] (* _ *).
+    (* Next Obligation. ex_t_solve_timeless. Qed. *)
 
     Definition Cell_inv_t : type (Z) :=
       na_ex_plain_t _ _ Cell_inv_t_inv_spec Cell_ty.
@@ -437,108 +429,86 @@ Section generated_code.
 
       lft_ctx -∗
       na_own π ⊤ -∗
-      maybe_creds true -∗
+      £ 1 -∗ (* Required: P.(na_inv_P) is not Timeless *)
+
       q.[κ] -∗
       l ◁ₗ[π, Shared κ] (#x) @ (◁ (∃na; P, ty)) ={F}=∗
 
-      ∃ r : rt, P.(na_inv_P) π r x ∗
-      l ◁ₗ[π, Owned true] PlaceIn r @ (◁ ty) ∗
+      ∃ r : rt,
+        P.(na_inv_P) π r x ∗
+        ▷ (l ◁ₗ[π, Owned false] PlaceIn r @ (◁ ty)) ∗
 
-      (* (∀ (r' : place_rfn rt), *)
-      ( l ◁ₗ[π, Owned false] (#r) @ (◁ ty) ={F}=∗
+        ( l ◁ₗ[π, Owned false] #r @ (◁ ty) ∗ P.(na_inv_P) π r x ={F}=∗
             q.[κ] ∗ na_own π ⊤ ).
     (* TODO: Closing view-shift here. *)
     Proof.
       iIntros (??) "#LFT Hna Hcred Hq #Hb".
-
       iEval (rewrite ltype_own_ofty_unfold /lty_of_ty_own) in "Hb".
       iDestruct "Hb" as (ly Halg Hly) "(Hsc & Hlb & %v & -> & #Hb)".
 
-      iMod (fupd_mask_mono with "Hb") as "#Hb'"; first done. iClear "Hb".
-
+      iMod (fupd_mask_mono with "Hb") as "#Hb'"; first done; iClear "Hb".
       iEval (unfold ty_shr, na_ex_plain_t) in "Hb'".
-      iDestruct "Hb'" as (r) "(HP & Hscr & Hbor & %ly' & %Hly' & %Halg')".
+      iDestruct "Hb'" as "(Hscr & Hbor & %ly' & %Hly' & %Halg')".
 
-      iMod (na_bor_acc with "LFT Hbor Hq Hna") as "(Hl & Hna & Hvs)"; [ solve_ndisj.. |].
+      iMod (na_bor_acc with "LFT Hbor Hq Hna") as "((%r & Hl & HP) & Hna & Hvs)"; [ solve_ndisj.. |].
+      iMod (lc_fupd_elim_later with "Hcred HP") as "HP".
 
       iModIntro; iExists r.
-      iSplitR; first done.
+      iSplitL "HP"; first done.
 
-      iSplitL "Hl Hcred".
+      iSplitL "Hl".
       { rewrite ltype_own_ofty_unfold /lty_of_ty_own.
-        iExists ly. iFrame (Halg Hly) "Hlb Hcred Hscr".
+        iExists ly => /=.
+        iFrame (Halg Hly) "Hlb Hscr"; iR.
         iExists r; iR.
         by iModIntro. }
 
-      iIntros "Hb".
-      iEval (rewrite ltype_own_ofty_unfold /lty_of_ty_own) in "Hb".
-      iDestruct "Hb" as (???) "(_ & #Hloc'' & _ & (% & -> & Hb)) /=".
+      iIntros "(Hl & HP)".
+      iEval (rewrite ltype_own_ofty_unfold /lty_of_ty_own) in "Hl".
+      iDestruct "Hl" as (???) "(_ & _ & _ & (%r' & -> & Hl)) /=".
+      iMod (fupd_mask_mono with "Hl") as "Hl"; first solve_ndisj.
 
-      (* iAssert (⌜ly0 = ly1⌝)%I as "<-". *)
-      (* { iPureIntro; by eapply syn_type_has_layout_inj. } *)
-
-      iMod (fupd_mask_mono with "Hb") as "Hb"; first done.
-      iApply ("Hvs" with "Hb Hna").
+      iApply ("Hvs" with "[Hl HP]"); last done.
+      iExists r'; iFrame.
     Qed.
 
     Lemma na_typed_place_ex_plain_t_shared π E L l (ty : type rt) x κ bmin K T :
-      li_tactic (lctx_lft_alive_count_goal E L κ)  (λ '(_, L2),
-        ∀ r, introduce_with_hooks E L2 (P.(na_inv_P) π r x)
-          (λ L3, typed_place π E L3 l
-                  (ShadowedLtype (◁ ty) #r (◁ (∃na; P, ty)))
-                  (#x) bmin (Owned true) K T))
+      prove_with_subtype E L false ProveDirect (£ 1) (λ L1 _ R, R -∗
+        li_tactic (lctx_lft_alive_count_goal E L1 κ)  (λ '(_, L2),
+          ∀ r, introduce_with_hooks E L2 (P.(na_inv_P) π r x)
+            (λ L3, typed_place π E L3 l
+                    (* TODO: (MagicLtype (◁ ty) (◁ (∃na; P, ty)) INV_MASK (λ mask rfn, P.(na_inv_P) π rfn x ∗ na_own π (⊤ minus ...)) (λ rfn, na_own π ⊤) (* TODO: Looks more OpenLTyped *) *)
+                    (ShadowedLtype (◁ ty) #r (◁ (∃na; P, ty)))
+                    (#x) bmin (Owned true) K T)))
       ⊢ typed_place π E L l (◁ (∃na; P, ty))%I (#x) bmin (Shared κ) K T.
     Proof.
-      rewrite /lctx_lft_alive_count_goal.
-      iIntros "(%κs & %L' & %Hal & HT)".
+      rewrite /prove_with_subtype.
+      iIntros "HT".
 
       rewrite /typed_place /introduce_with_hooks.
-      iIntros (Φ ???) "#(LFT & TIME & LLCTX) #HE HL Hincl Hb Hcont".
-
+      iIntros (Φ ???) "#(LFT & TIME & LLCTX) #HE HL Hincl Hl Hcont".
       iApply fupd_place_to_wp.
-      iMod (lctx_lft_alive_count_tok with "HE HL") as (q) "(Htok & Htokcl & HL)"; [ done.. |].
-      iMod (na_ex_plain_t_open_shared with "LFT [] [] Htok Hb") as (r) "(HP & Hb & Hvs)"; [ done.. | admit | admit |].
 
-      iMod ("HT" with "[] HE HL HP") as "(%L2 & HL & HT)"; first done.
-      iApply ("HT" with "[//] [//] [$LFT $TIME $LLCTX] HE HL [Hincl] [Hb]").
+      iMod ("HT" with "[] [] [$LFT $TIME $LLCTX] HE HL")
+          as "(% & % & % & >(Hcred & HR) & HL & HT)"; [ solve_ndisj.. |].
+      iSpecialize ("HT" with "HR").
+
+      rewrite /li_tactic /lctx_lft_alive_count_goal.
+      iDestruct "HT" as "(% & % & %Hal & HT)".
+
+      iMod (lctx_lft_alive_count_tok with "HE HL") as (q) "(Htok & Htokcl & HL)"; [ solve_ndisj | done |].
+      iMod (na_ex_plain_t_open_shared with "LFT [] Hcred Htok Hl") as (r) "(HP & Hl & Hvs)"; [ done.. | |].
+      { (* TODO: Correctly pass na_own π ⊤ *) admit. }
+
+      iMod ("HT" with "[] HE HL HP") as "(% & HL & HT)"; first done.
+      iApply ("HT" with "[//] [//] [$LFT $TIME $LLCTX] HE HL [Hincl] [Hl]").
       { by iApply (bor_kind_incl_trans with "Hincl"). }
-      { rewrite ltype_own_shadowed_unfold /shadowed_ltype_own; iR.
-        iEval (rewrite ltype_own_ofty_unfold /lty_of_ty_own) in "Hb".
-
-        iDestruct "Hb" as (ly) "(#Hsyn & #Hly & #Hsc & #Hlb & _ & Hb)".
-        iDestruct "Hb" as (r') "(#Hrfn & Hb)" => /=.
-
-        iSplitL; rewrite ltype_own_ofty_unfold /lty_of_ty_own.
-        - iExists ly; iFrame "#".
-          iSplitR; first admit.
-          iExists r'; iFrame "# ∗".
-
-        - iExists ly; iFrame "#".
-          iSplitR; first admit.
-          iExists x; iR.
-          simpl. admit. }
+      { admit. }
 
       iModIntro.
       iIntros (L'' κs' l2 b2 bmin0 rti ltyi ri strong weak) "Hincl Hl Hc".
       iApply ("Hcont" with "Hincl Hl").
-
-      iSplit.
-      - iDestruct "Hc" as "[Hc _]".
-        simp_ltypes; destruct strong; last done.
-
-        iIntros (r' r'' κs'') "Hl %".
-        iSpecialize ("Hc" $! r' r'' κs'').
-
-        admit.
-
-      - iDestruct "Hc" as "[_ Hc]".
-        destruct weak; last done.
-        iIntros (???) "Hincl Hl Hcond".
-        iMod ("Hc" with "Hincl Hl Hcond") as "(Ha & Hb & Htoks & Hc)".
-        iFrame.
-        iDestruct "Hb" as "(Hcond_ty & _)".
-
-        admit.
+      admit.
     Admitted.
   End na_subtype.
 
